First few tactics to automate the proof of one-step computational strategies

sources/Abstract/Strategies.v
@@ -21,31 +21,31 @@ Section Strategy.
   | Par : (nat -> stg) -> nat -> nat -> stg
   | Hole : group -> stg.
 
-  Fixpoint interp (s : stg) : group :=
+  Fixpoint shape (s : stg) : group :=
     match s with
-      | Seq s1 s2 => interp s1 ∪ interp s2
-      | Loop s a b => (⋃⎨interp (s i), i ∈〚a, b〛⎬)
-      | Par s a b => (⋃⎨interp (s i), i ∈〚a, b〛⎬)
+      | Seq s1 s2 => shape s1 ∪ shape s2
+      | Loop s a b => (⋃⎨shape (s i), i ∈〚a, b〛⎬)
+      | Par s a b => (⋃⎨shape (s i), i ∈〚a, b〛⎬)
       | Hole g => g
     end.
 
   Fixpoint PO (s : stg) (A : group) : Prop :=
     match s with
       | Seq s1 s2 =>
-        PO s1 A /\ PO s2 (A ∪ interp s1)
+        PO s1 A /\ PO s2 (A ∪ shape s1)
       | Loop s a b =>
         a <= b /\ PO (s a) A /\
-        forall i, a <= i < b -> PO (s (1+i)) (A ∪ interp (Loop s a i))
+        forall i, a <= i < b -> PO (s (1+i)) (A ∪ shape (Loop s a i))
       | Par s a b =>
         a <= b /\ forall i, a <= i <= b -> PO (s i) A
       | Hole g => valid _ A g
     end.
 
   Lemma PO_sound :
-    forall s A, PO s A -> valid _ A (A ∪ (interp s)).
+    forall s A, PO s A -> valid _ A (A ∪ (shape s)).
   Proof.
     induction s; intros; simpl in *.
-    + apply sequ with (A ∪ interp s1).
+    + apply sequ with (A ∪ shape s1).
       * firstorder.
       * rewrite <- union_assoc; now apply IHs2.
     + apply loop; [firstorder|firstorder|].
@@ -56,6 +56,36 @@ Section Strategy.
     + apply par; firstorder.
     + now apply append.
   Qed.
+
+  (** Now we turn to refinement of abstract strategies. *)
+
+  Inductive refines : stg -> stg -> Prop :=
+  | refines_seq :
+      forall s1 s2 s1' s2',
+        refines s1 s1' -> refines s2 s2' -> refines (Seq s1 s2) (Seq s1' s2')
+  | refines_loop :
+      forall s1 s2 a b, (forall i, a <= i <= b -> refines (s1 i) (s2 i)) ->
+                        refines (Loop s1 a b) (Loop s2 a b)
+  | refines_par :
+      forall s1 s2 a b, (forall i, a <= i <= b -> refines (s1 i) (s2 i)) ->
+                        refines (Par s1 a b) (Par s2 a b)
+  | refines_hole :
+      forall s g, shape s = g -> refines s (Hole g).
+
+  Inductive computational : stg -> Prop :=
+  | comp_seq :
+      forall s1 s2,
+        computational s1 -> computational s2 -> computational (Seq s1 s2)
+  | comp_loop :
+      forall s a b,
+        (forall i, a <= i <= b -> computational (s i)) ->
+        computational (Loop s a b)
+  | comp_par :
+      forall s a b,
+        (forall i, a <= i <= b -> computational (s i)) ->
+        computational (Par s a b)
+  | comp_hole :
+      forall g, singleton g -> computational (Hole g).
 End Strategy.
 
 Delimit Scope stg_scope with stg.
