examples/VonNeumann1D.v
@@ -1,0 +1,61 @@
+Require Import StLib.Core.
+
+Section VonNeumann1D.
+  Variables n : nat.
+  Variable T : nat.
+
+  Instance VonNeumann1D : Stencil nat1 :=
+  {
+    space   := 〚0, n-1〛;
+    nb_iter := T;
+    pattern := [0; 1; 2];
+    center  := 1
+  }.
+End VonNeumann1D.
+
+Section Triangle.
+  Variable n : nat.
+
+  Definition compute_triangle :=
+    (For i ∈〚0, n-1〛Do
+         Compute 〚i, 2 * n - 1 - i〛× ⎨i⎬).
+
+  Eval simpl in (shape compute_triangle).
+
+  Tactic Notation "destruct" "pairs" :=
+    repeat match goal with
+             | [ x : @prod _ _ |- _ ] => destruct x
+           end.
+
+  Tactic Notation "generate" "proof" "obligations" :=
+    apply PO_sound; simpl; firstorder.
+
+  Tactic Notation "one" "step" :=
+    unfold valid, closure;
+    union with 1; unfold iter_next, next;
+
+    match goal with
+      | [ |- @is_in _ ?x (@union _ (@image _ _
+          (@finite _ (@cons _ ?A (@nil _))) _))] =>
+        union with A; firstorder;
+        image with x;[|apply same_eq; firstorder]
+    end;
+
+    unfold boundary, extension, subset; firstorder;
+    destruct pairs; simpl in *; subst;
+    sets simpl;
+
+    match goal with
+      | [ H : depends _ _ _ |- _ ] => inversion H; clear H
+    end.
+
+
+  Lemma compute_triangle_valid :
+    ∅ ⟿ ∅ ∪ shape compute_triangle // VonNeumann1D (2 * n) n.
+  Proof.
+    generate proof obligations.
+    + one step.
+    + unfold valid, closure.
+      union with 1; unfold iter_next, next.
+  Abort.
+End Triangle.
