sources/Core.v
@@ -3,5 +3,7 @@ Require Export Common.Sets Common.Monoids Common.Stencils
 Require Export List.
 
 Open Scope set_scope.
+Open Scope sem_scope.
 Open Scope stg_scope.
+Open Scope monoid.
 Export ListNotations.
