Makefile
@@ -10,7 +10,7 @@ SOURCES_VS  := $(SOURCES_MODULES:%=sources/%.v)
 SOURCES_VOS := $(SOURCES_MODULES:%=sources/%.vo)
 
 EXAMPLES_MODULES := \
-	First
+	VonNeumann1D
 EXAMPLES_VS  := $(EXAMPLES_MODULES:%=examples/%.v)
 EXAMPLES_VOS := $(EXAMPLES_MODULES:%=examples/%.vo)
 
